Added definitions and rules for choice with dependent binders

multi_actris/channel/channel.v
@@ -130,6 +130,23 @@ Definition chan_pool `{!heapGS Σ, !chanG Σ}
             own (γEs !!! i) (◯E (Next p)) ∗
             iProto_own γ i p).
 
+Definition sum_reduce {A B C} (f1 : A → C) (f2 : B → C) (ab : A + B) : C :=
+  match ab with
+  | inl a => f1 a
+  | inr b => f2 b
+  end.
+
+Definition iProto_choice {Σ} {TT1 TT2 : tele}
+           (a:action)
+           (v1 : TT1 → val) (v2 : TT2 → val)
+           (P1 : TT1 → iProp Σ) (P2 : TT2 → iProp Σ)
+           (p1 : TT1 → iProto Σ) (p2 : TT2 → iProto Σ) : iProto Σ :=
+  (<a @ (tt: TT1 + TT2)> MSG (sum_reduce (InjLV ∘ v1) (InjRV ∘ v2) tt)
+    {{ sum_reduce P1 P2 tt }} ; sum_reduce p1 p2 tt)%proto.
+Global Typeclasses Opaque iProto_choice.
+Arguments iProto_choice {_ _ _} _ _ _ _%I _%I _%proto _%proto.
+Global Instance: Params (@iProto_choice) 4 := {}.
+
 Section channel.
   Context `{!heapGS Σ, !chanG Σ}.
   Implicit Types p : iProto Σ.
@@ -474,6 +491,121 @@ Section channel.
     { iRight. iRight. iExists _. iFrame. }
     wp_pure _.
     rewrite iMsg_base_eq iMsg_exist_eq.
+    iDestruct "Hm" as (x <-) "[Hp HP]".
+    wp_pures.
+    iMod (own_update_2 with "H● H◯") as "[H● H◯]";[apply excl_auth_update|].
+    iModIntro. iApply "HΦ".
+    iFrame. iExists _, _, _, _, _, _. iSplit; [done|].
+    iRewrite "Hp". iFrame "#∗". iApply iProto_le_refl.
+  Qed.
+
+  Lemma iProto_le_select_l {TT1 TT2:tele} j
+        (v1 : TT1 → val) (v2 : TT2 → val) P1 P2 (p1 : TT1 → iProto Σ) (p2 : TT2 → iProto Σ) :
+    ⊢ (iProto_choice (Send, j) v1 v2 P1 P2 p1 p2) ⊑
+      (<(Send,j) @.. (tt:TT1)> MSG (InjLV (v1 tt)) {{ P1 tt }} ; p1 tt).
+  Proof.
+    rewrite /iProto_choice.
+    iApply iProto_le_trans; last first.
+    { iApply iProto_le_texist_elim_r. iIntros (x). iExists x.
+      iApply iProto_le_refl. }
+    iIntros (tt). by iExists (inl tt).
+  Qed.
+
+  Lemma iProto_le_select_r {TT1 TT2:tele} j
+        (v1 : TT1 → val) (v2 : TT2 → val) P1 P2 (p1 : TT1 → iProto Σ) (p2 : TT2 → iProto Σ) :
+    ⊢ (iProto_choice (Send, j) v1 v2 P1 P2 p1 p2) ⊑
+      (<(Send,j) @.. (tt:TT2)> MSG (InjRV (v2 tt)) {{ P2 tt }} ; p2 tt).
+  Proof.
+    rewrite /iProto_choice.
+    iApply iProto_le_trans; last first.
+    { iApply iProto_le_texist_elim_r. iIntros (x). iExists x.
+      iApply iProto_le_refl. }
+    iIntros (tt). by iExists (inr tt).
+  Qed.
+
+  Lemma select_spec_tele {TT1 TT2:tele} (tt:TT1 + TT2) c j
+        (v1 : TT1 → val) (v2 : TT2 → val) P1 P2 (p1 : TT1 → iProto Σ) (p2 : TT2 → iProto Σ) :
+    {{{ c ↣ (iProto_choice (Send, j) v1 v2 P1 P2 p1 p2) ∗
+      sum_reduce P1 P2 tt }}}
+       send c #j (Val (sum_reduce (InjLV ∘ v1) (InjRV ∘ v2) tt))
+    {{{ RET #(); c ↣ (sum_reduce p1 p2 tt) }}}.
+  Proof.
+    iIntros (Φ) "[Hc HP] HΦ".
+    destruct tt.
+    - iDestruct (iProto_pointsto_le with "Hc []") as "Hc".
+      { iApply iProto_le_select_l. }
+      simpl.
+      replace (InjLV (v1 t)) with ((InjLV ∘ v1) t) by done.
+      by iApply (send_spec_tele with "[$Hc $HP]").
+    - iDestruct (iProto_pointsto_le with "Hc []") as "Hc".
+      { iApply iProto_le_select_r. }
+      simpl.
+      replace (InjRV (v2 t)) with ((InjRV ∘ v2) t) by done.
+      by iApply (send_spec_tele with "[$Hc $HP]").
+  Qed.
+
+  (* OBS: Can we reuse recv_spec here? *)
+  Lemma branch_spec_tele {TT1 TT2:tele} c j
+        (v1 : TT1 → val) (v2 : TT2 → val) P1 P2 (p1 : TT1 → iProto Σ) (p2 : TT2 → iProto Σ) :
+    {{{ c ↣ (iProto_choice (Recv, j) v1 v2 P1 P2 p1 p2) }}}
+       recv c #j
+    {{{ (tt:TT1 + TT2), RET (sum_reduce (InjLV ∘ v1) (InjRV ∘ v2) tt);
+            c ↣ (sum_reduce p1 p2 tt) ∗ sum_reduce P1 P2 tt }}}.
+  Proof.
+    iIntros (Φ) "Hc HΦ". iLöb as "HL". wp_lam.
+    rewrite iProto_pointsto_eq.
+    iDestruct "Hc" as
+      (γ γE l i n p' ->) "(#IH & #Hls & Hle & H● & H◯ & Hown)".
+    do 6 wp_pure _. wp_bind (Fst _). wp_pure _.
+    iInv "IH" as "Hctx".
+    iDestruct (iProto_le_msg_inv_r with "Hle") as (m') "#Heq".
+    iRewrite "Heq" in "Hown".
+    iAssert (▷ (⌜i < n⌝ ∗ iProto_own γ i (<(Recv, j)> m') ∗
+                iProto_ctx γ n))%I with "[Hctx Hown]"
+      as "[Hi [Hown Hctx]]".
+    { iNext. iDestruct (iProto_ctx_agree with "Hctx Hown") as %Hi.
+      iFrame. done. }
+    iAssert (▷ (▷ ⌜j < n⌝ ∗ iProto_own γ i (<(Recv, j)> m') ∗
+                iProto_ctx γ n))%I with "[Hctx Hown]" as "[Hj [Hown Hctx]]".
+    { iNext. iDestruct (iProto_target with "Hctx Hown") as "[Hin [$$]]".
+      iFrame. }
+    iRewrite -"Heq" in "Hown". wp_pures. iModIntro. iFrame.
+    wp_smart_apply (vpos_spec); [done|]; iIntros "_".
+    iDestruct "Hi" as %Hi.
+    iDestruct "Hj" as %Hj.
+    iDestruct ("Hls" $! j i with "[//] [//]") as (γt) "IHl2".
+    wp_pures.
+    wp_bind (Xchg _ _).
+    iInv "IHl2" as "HIp".
+    iDestruct "HIp" as "[HIp|HIp]".
+    { iDestruct "HIp" as ">[Hl' Htok]".
+      wp_xchg. iModIntro.
+      iSplitL "Hl' Htok".
+      { iLeft. iFrame. }
+      wp_pures. iApply ("HL" with "[H● H◯ Hown Hle] HΦ").
+      iExists _, _, _, _, _, _. iSplit; [done|]. iFrame "#∗". }
+    iDestruct "HIp" as "[HIp|HIp]"; last first.
+    { iDestruct "HIp" as (p'') "[>Hl' [Hown' H◯']]".
+      wp_xchg.
+      iModIntro.
+      iSplitL "Hl' Hown' H◯'".
+      { iRight. iRight. iExists _. iFrame. }
+      wp_pures. iApply ("HL" with "[H● H◯ Hown Hle] HΦ").
+      iExists _, _, _, _, _, _. iSplit; [done|]. iFrame "#∗". }
+    iDestruct "HIp" as (w m p'') "(>Hl' & Hown' & Hm & Hp')".
+    iInv "IH" as "Hctx".
+    wp_xchg.
+    iDestruct (iProto_own_le with "Hown Hle") as "Hown".
+    iMod (iProto_step with "Hctx Hown' Hown Hm") as
+      (p''') "(Hm & Hctx & Hown & Hown')".
+    iModIntro.
+    iSplitL "Hctx"; [done|].
+    iModIntro.
+    iSplitL "Hl' Hown Hp'".
+    { iRight. iRight. iExists _. iFrame. }
+    wp_pure _.
+    rewrite iMsg_base_eq.
+    rewrite iMsg_exist_eq.
     iDestruct "Hm" as (x <-) "[Hp HP]".
     wp_pures.
     iMod (own_update_2 with "H● H◯") as "[H● H◯]";[apply excl_auth_update|].
